working on D major test

src/AddTest.v
@@ -64,7 +64,7 @@ Definition add_one_body : Emajor.stmt :=
                         ::nil) (Var arg)).
 
 Definition add_one_fn : Emajor.function :=
-  Emajor.mkfunction (add_one_id :: arg :: nil) 8%Z (add_one_body,Var ans).
+  Emajor.mkfunction (add_one_id :: arg :: nil) EMsig 8%Z (add_one_body,Var ans).
 
 
 Definition main_body : Emajor.stmt :=
@@ -75,8 +75,11 @@ Definition main_body : Emajor.stmt :=
        (Emajor.Sseq (Emajor.SmakeConstr main_tmp1 (Int.repr tag_S) ((Var main_tmp0)::nil))
                     (Emajor.Scall main_tmp2 (Var add_one_id) (Var main_tmp1)))).
 
+Definition main_sig :=
+  mksignature [] (Some Tint) cc_default.
+
 Definition main_fn : Emajor.function :=
-  Emajor.mkfunction nil
+  Emajor.mkfunction nil main_sig
                     16%Z (main_body,Var main_tmp2).
 
 Definition add_one_prog : Emajor.program :=
@@ -89,16 +92,12 @@ Definition cM := Dmajortocmajor.transf_prog dM.
 Definition cm := Cmajortominor.transf_prog cM.
 Definition asm := transf_cminor_program cm.
 
-(* Now we need to extract all of this *)
-(* in order to run it *)
-(* I'm not sure how to do that *)
-
-Definition i := initial_state add_one_prog.
 
 Ltac take_step :=
   eapply star_step;
   match goal with
   | [ |- step _ _ _ _ ] => econstructor; eauto
+  | [ |- Dmajor.step _ _ _ _ ] => econstructor; eauto
   | [ |- E0 = _ ** _ ] => replace E0 with (E0 ** E0) by (simpl; reflexivity);
                             reflexivity
   | [ |- eval_expr _ _ _ ] => solve [simpl; instantiate; econstructor; eauto; simpl; try reflexivity]
@@ -107,7 +106,200 @@ Ltac take_step :=
   end.
 
 
-Lemma add_one_prog_step :
+Lemma add_one_prog_step_D_major :
+  forall s,
+    Dmajor.initial_state dM s ->
+    exists s',
+      star (Dmajor.step) (Genv.globalenv dM) s E0 s'.
+Proof.
+  intros.
+  unfold dM in *.
+  simpl in *.
+  eexists.
+  unfold add_one_prog in *.
+  inv H.
+  simpl in *.
+  subst ge.
+  remember Emajortodmajor.transf_prog as tp.
+  rewrite Heqtp in H1. unfold Emajortodmajor.transf_prog in *.
+  simpl in H1. unfold Genv.find_symbol in H1.
+  simpl in H1. inv H1.
+  clear H1.
+  unfold Emajortodmajor.transf_prog in *.
+  simpl in H2. unfold Genv.find_funct_ptr in H2.
+  simpl in H2. inv H2.
+  clear H2.
+  simpl in *.
+
+  clear H.
+  unfold Genv.init_mem in *.
+  simpl in *.
+  repeat (break_match_hyp; try congruence).
+  invc H0.
+  unfold EMsig in *. unfold signature_main in *.
+  clear H3. 
+
+  destruct (Mem.alloc m0 0 16) eqn:?. 
+  take_step.
+  take_step.
+  take_step.
+  take_step.
+  take_step.
+  destruct (Mem.alloc m1 (-4) (Int.unsigned (Int.repr 4))) eqn:?.
+  destruct (Mem.store Mint32 m4 b2 (-4) (Vint (Int.repr 4))) eqn:?.
+  take_step.
+  simpl.
+  econstructor; eauto.
+  simpl. reflexivity.
+  simpl. econstructor; eauto.
+  Focus 2. admit. (* mem store must work, bring from alloc fact *)
+  (* threading memory through here will be ugly *)
+  
+
+  take_step.
+  destruct (Mem.storev Mint32 m5 (Vptr b2 Int.zero) (Vptr 1%positive Int.zero)) eqn:?. Focus 2. admit.
+  take_step.
+  simpl. econstructor. simpl. reflexivity.
+  simpl. econstructor. simpl. reflexivity.
+
+  take_step.
+  take_step.
+  take_step.
+  take_step.
+  take_step.
+  destruct (Mem.alloc m6 (-4) (Int.unsigned (Int.repr 4))) eqn:?. 
+  destruct (Mem.store Mint32 m7 b3 (-4) (Vint (Int.repr 4))) eqn:?.
+  Focus 2. admit.
+  take_step.
+  simpl. econstructor; eauto. simpl. reflexivity.
+  simpl. econstructor; eauto.
+
+  take_step.
+
+  destruct (Mem.storev Mint32 m8 (Vptr b3 Int.zero) (Vint (Int.repr tag_0))) eqn:?.
+  Focus 2. admit.
+  take_step.
+  econstructor; eauto.
+  econstructor; eauto.
+
+  take_step.
+  take_step.
+  take_step.
+  take_step.
+  take_step.
+
+  destruct (Mem.alloc m9 (-4)
+                      (Int.unsigned (Int.repr (4 + 4 * Z.of_nat (length [Var main_tmp0]))))) eqn:?.
+  destruct (Mem.store Mint32 m10 b4 (-4)
+                      (Vint (Int.repr (4 + 4 * Z.of_nat (length [Var main_tmp0]))))) eqn:?.
+  Focus 2. admit.
+  take_step.
+
+  econstructor; eauto.
+  econstructor; eauto.
+  econstructor; eauto.
+
+  take_step.
+
+  destruct (Mem.storev Mint32 m11 (Vptr b4 Int.zero) (Vint (Int.repr tag_S))) eqn:?.
+  Focus 2. admit.
+  
+  take_step.
+  econstructor; eauto. simpl. 
+  econstructor; eauto. simpl.
+
+  take_step.
+  take_step.
+
+
+  destruct (Mem.storev Mint32 m12 (Val.add (Vptr b4 Int.zero) (Vint (Int.repr 4)))
+     (Vptr b3 Int.zero)) eqn:?. Focus 2. admit.
+  take_step.
+  econstructor; eauto.
+  econstructor; eauto. simpl. 
+  econstructor; eauto. simpl. 
+  econstructor; eauto. simpl.
+
+  take_step.
+  take_step.
+
+  assert (Mem.loadv Mint32 m13 (Vptr b2 Int.zero) = Some (Vptr 1%positive Int.zero)) by admit.
+  simpl.
+  take_step.
+  simpl. econstructor; eauto.
+  econstructor; eauto. simpl.
+  econstructor; eauto. econstructor; eauto. simpl. reflexivity.
+  econstructor; eauto.
+  econstructor; eauto.
+  simpl. reflexivity.
+  econstructor; eauto.
+  simpl. break_match; try congruence.
+  unfold Genv.find_funct_ptr. simpl. reflexivity.
+  simpl. reflexivity.
+
+  destruct (Mem.alloc m13 0
+                      (Dmajor.fn_stackspace (Emajortodmajor.transf_fundef add_one_fn))) eqn:?.
+
+  take_step.
+  simpl.
+  take_step.
+  take_step.
+  simpl.
+  take_step.
+  take_step.
+  destruct (Mem.alloc m14 (-4) (Int.unsigned (Int.repr 4))) eqn:?.
+  destruct (Mem.store Mint32 m15 b6 (-4) (Vint (Int.repr 4))) eqn:?.
+  Focus 2. admit.
+  take_step.
+  econstructor; eauto.
+  econstructor; eauto.
+  econstructor; eauto.
+  take_step.
+
+  destruct (Mem.store Mint32 m16 b6 (Int.unsigned Int.zero) (Vptr 1%positive Int.zero)) eqn:?.
+  Focus 2. admit.
+  
+  take_step.
+
+  econstructor; eauto.
+  simpl. reflexivity.
+  econstructor; eauto. econstructor; eauto.
+  simpl. eauto.
+
+  take_step.
+  take_step.
+  take_step.
+  take_step.
+  take_step.
+  take_step.
+  take_step.
+  assert (Mem.loadv Mint32 m17 (Vptr b4 Int.zero) = Some (Vint (Int.repr tag_S))) by admit.
+  take_step.
+  econstructor; eauto.
+  econstructor; eauto.
+  
+  take_step.
+  take_step.
+  econstructor; eauto.
+  econstructor; eauto.
+  unfold tag_S. econstructor; eauto.
+
+
+(* HERE *)
+  take_step.
+  take_step.
+  take_step.
+  take_step.
+  take_step.
+  take_step.
+  econstructor; eauto. simpl.
+  
+Admitted.
+  
+  
+Definition i := initial_state add_one_prog.
+
+Lemma add_one_prog_step_E_major :
   forall s,
     i s ->
     star step (Genv.globalenv add_one_prog) s E0
